Move part of SubstVar to a new VarsOfExpr module

src/Transforms/SubstVar.dfy
@@ -6,6 +6,7 @@ include "../Semantics/ExprInduction.dfy"
 include "../Semantics/InterpStateIneq.dfy"
 include "../Semantics/EqInterpRefl.dfy"
 include "../Semantics/Pure.dfy"
+include "VarsOfExpr.dfy"
 
 module Bootstrap.Transforms.SubstVar.Subst.Base {
   import opened AST.Syntax
@@ -17,89 +18,12 @@ module Bootstrap.Transforms.SubstVar.Subst.Base {
   import opened Semantics.Pure
   import opened Generic
   import Shallow
+  import opened VarsOfExpr
 
   type Environment = Interp.Environment
   type State = Interp.State
   type Expr = Interp.Expr
 
-  function method {:opaque} SeqToSet<T>(s: seq<T>): set<T>
-    // Unfortunately, we need this small opaque helper to prevent with proof explosions.
-  {
-    set x | x in s
-  }
-
-  function method {:opaque} VarsToNameSet(vars: seq<Exprs.TypedVar>): set<string>
-    // Same as for ``SeqToSet``: making this definition opaque is annoying, but we need it to
-    // prevent proof explosions.
-  {
-    set x | x in vars :: x.name
-  }
-
-  // TODO(SMH): move?
-  function method VarsOfExpr(read: bool, e: Syntax.Expr): set<string>
-    decreases e.Size(), 0
-    // Return the set of all variables used in an expression (accessed, updated or even declared).
-    //
-    // `read`: if true, include in the set the variables which are read, otherwise ignore them.
-  {
-    reveal Interp.SupportsInterp();
-    match e {
-      case Var(v) => if read then {v} else {}
-      case Literal(_) => {}
-      case Abs(vars, body) =>
-        (set x | x in vars) + VarsOfExpr(read, body)
-      case Apply(aop, exprs) =>
-        VarsOfExprs(read, exprs)
-      case Block(exprs) =>
-        VarsOfExprs(read, exprs)
-      case VarDecl(vdecls, ovals) =>
-        var s := if ovals.Some? then VarsOfExprs(read, ovals.value) else {};
-        s + VarsToNameSet(vdecls)
-      case Update(vars, vals) =>
-        (set x | x in vars) + VarsOfExprs(read, vals)
-      case Bind(vars, vals, body) =>
-        VarsToNameSet(vars) + VarsOfExprs(read, vals) + VarsOfExpr(read, body)
-      case If(cond, thn, els) =>
-        VarsOfExpr(read, cond) + VarsOfExpr(read, thn) + VarsOfExpr(read, els)
-    }
-  }
-
-  function method VarsOfExprs(read: bool, es: seq<Syntax.Expr>): set<string>
-    decreases Expr.Exprs_Size(es), 1
-  {
-    if es == [] then {}
-    else VarsOfExpr(read, es[0]) + VarsOfExprs(read, es[1..])
-  }
-
-  function method UpdtVarsOfExpr(e: Syntax.Expr): set<string>
-  {
-    VarsOfExpr(false, e)
-  }
-
-  function method UpdtVarsOfExprs(es: seq<Syntax.Expr>): set<string>
-  {
-    VarsOfExprs(false, es)
-  }
-
-  function method AllVarsOfExpr(e: Syntax.Expr): set<string>
-  {
-    VarsOfExpr(true, e)
-  }
-
-  function method AllVarsOfExprs(es: seq<Syntax.Expr>): set<string>
-  {
-    VarsOfExprs(true, es)
-  }
-
-  // Accumulator used for substitutions.
-  // `subst`: the substitution
-  // `frozen`: the variables which appear in the expressions with which we substitute
-  datatype SubstAcc = SubstAcc(subst: map<string, Expr>)//, frozen: set<string>)
-
-  predicate method NotVarDecl(e: Syntax.Expr)
-  {
-    !e.VarDecl?
-  }
     
   function method SubstInExpr(acc: SubstAcc, e: Expr): (e':Expr)
     decreases e.Size(), 0
@@ -178,6 +102,7 @@ module Bootstrap.Transforms.SubstVar.Subst.Base {
 module Bootstrap.Transforms.SubstVar.Subst.BaseProofs refines Semantics.ExprInduction {
   import opened Semantics.Pure
   import opened Base
+  import opened VarsOfExpr
   import Semantics.InterpStateIneq
   import Semantics.EqInterpRefl
 
