src/Transforms/VarsOfExpr.dfy
@@ -1,0 +1,120 @@
+include "../Utils/Library.dfy"
+include "../Utils/StrTree.dfy"
+include "../Semantics/Interp.dfy"
+include "../Semantics/Equiv.dfy"
+include "../Semantics/ExprInduction.dfy"
+include "../Semantics/InterpStateIneq.dfy"
+include "../Semantics/EqInterpRefl.dfy"
+include "../Semantics/Pure.dfy"
+
+// TODO(SMH): I wanted to name this: `Bootstrap.Transforms.VarsOfExpr.Base`,
+// and have a module `Bootstrap.Transforms.VarsOfExpr.Proofs`, but this causes
+// trouble in `Bootstrap.Transforms.SubstVar.Subst.Proofs`, because I then want to
+// to `import opened VarsOfExpr.Base`, but it conflicts with the
+// `import opened Bootstrap.Transforms.SubstVar.Subst.Base`...
+module Bootstrap.Transforms.VarsOfExpr {
+  import opened AST.Syntax
+  import opened Utils.Lib
+  import opened Utils.Lib.Datatypes
+  import opened AST.Predicates
+  import Semantics.Interp
+  import opened Semantics.Equiv
+  import opened Semantics.Pure
+  import opened Generic
+  import Shallow
+
+  type Environment = Interp.Environment
+  type State = Interp.State
+  type Expr = Interp.Expr
+
+  function method {:opaque} SeqToSet<T>(s: seq<T>): set<T>
+    // Unfortunately, we need this small opaque helper to prevent with proof explosions.
+  {
+    set x | x in s
+  }
+
+  function method {:opaque} VarsToNameSet(vars: seq<Exprs.TypedVar>): set<string>
+    // Same as for ``SeqToSet``: making this definition opaque is annoying, but we need it to
+    // prevent proof explosions.
+  {
+    set x | x in vars :: x.name
+  }
+
+  // TODO(SMH): move?
+  function method VarsOfExpr(read: bool, e: Syntax.Expr): set<string>
+    decreases e.Size(), 0
+    // Return the set of all variables used in an expression (accessed, updated or even declared).
+    //
+    // `read`: if true, include in the set the variables which are read, otherwise ignore them.
+  {
+    reveal Interp.SupportsInterp();
+    match e {
+      case Var(v) => if read then {v} else {}
+      case Literal(_) => {}
+      case Abs(vars, body) =>
+        (set x | x in vars) + VarsOfExpr(read, body)
+      case Apply(aop, exprs) =>
+        VarsOfExprs(read, exprs)
+      case Block(exprs) =>
+        VarsOfExprs(read, exprs)
+      case VarDecl(vdecls, ovals) =>
+        var s := if ovals.Some? then VarsOfExprs(read, ovals.value) else {};
+        s + VarsToNameSet(vdecls)
+      case Update(vars, vals) =>
+        (set x | x in vars) + VarsOfExprs(read, vals)
+      case Bind(vars, vals, body) =>
+        VarsToNameSet(vars) + VarsOfExprs(read, vals) + VarsOfExpr(read, body)
+      case If(cond, thn, els) =>
+        VarsOfExpr(read, cond) + VarsOfExpr(read, thn) + VarsOfExpr(read, els)
+    }
+  }
+
+  function method VarsOfExprs(read: bool, es: seq<Syntax.Expr>): set<string>
+    decreases Expr.Exprs_Size(es), 1
+  {
+    if es == [] then {}
+    else VarsOfExpr(read, es[0]) + VarsOfExprs(read, es[1..])
+  }
+
+  function method UpdtVarsOfExpr(e: Syntax.Expr): set<string>
+  {
+    VarsOfExpr(false, e)
+  }
+
+  function method UpdtVarsOfExprs(es: seq<Syntax.Expr>): set<string>
+  {
+    VarsOfExprs(false, es)
+  }
+
+  function method AllVarsOfExpr(e: Syntax.Expr): set<string>
+  {
+    VarsOfExpr(true, e)
+  }
+
+  function method AllVarsOfExprs(es: seq<Syntax.Expr>): set<string>
+  {
+    VarsOfExprs(true, es)
+  }
+
+  // Accumulator used for substitutions.
+  // `subst`: the substitution
+  // `frozen`: the variables which appear in the expressions with which we substitute
+  datatype SubstAcc = SubstAcc(subst: map<string, Expr>)//, frozen: set<string>)
+
+  predicate method NotVarDecl(e: Syntax.Expr)
+  {
+    !e.VarDecl?
+  }
+}
+
+// Rem.(SMH): about the name, see the comment for `Bootstrap.Transforms.VarsOfExpr`
+module Bootstrap.Transforms.VarsOfExprUselessBindings.Base {
+  // This module proves that:
+  // If:
+  // - we have an expression `e` and contexts `ctx` and `ctx'`
+  // - `ctx'` is `ctx` augmented with bindings which don't appear in `e`
+  // Then:
+  // - evaluating `e` starting from `ctx` and `ctx'` leads to similar results
+
+  
+}
